Output a resulting cx val

src/dynamics.lean
@@ -1,16 +1,16 @@
 import syntax
 
-inductive steps: cx val -> exp -> exp -> Prop
+inductive steps: cx val -> exp -> cx val -> exp -> Prop
 | if_e1
-    (Δ: cx val)
+    (Δ: cx val) (Δ': cx val)
     (e1: exp) (e1': exp) (e2: exp) (e3: exp):
-    steps Δ e1 e1' ->
-    steps Δ (exp.if_ e1 e2 e3) (exp.if_ e1' e2 e3)
+    steps Δ e1 Δ' e1' ->
+    steps Δ (exp.if_ e1 e2 e3) Δ' (exp.if_ e1' e2 e3)
 | if_true
     (Δ: cx val)
     (e2: exp) (e3: exp):
-    steps Δ (exp.if_ (exp.pure val.true) e2 e3) e2
+    steps Δ (exp.if_ (exp.pure val.true) e2 e3) Δ e2
 | if_false
     (Δ: cx val)
     (e2: exp) (e3: exp):
-    steps Δ (exp.if_ (exp.pure val.false) e2 e3) e3
+    steps Δ (exp.if_ (exp.pure val.false) e2 e3) Δ e3
